floyd/SeparationLogicAsLogicSoundness.v
@@ -214,7 +214,7 @@ Theorem semax_prog_rule :
        forall n,
          { jm |
            m_dry jm = m /\ level jm = n /\
-           nth_error (ghost_of (m_phi jm)) 0 = Some (Some (ext_ghost z, NoneP)) /\
+           nth_error (ghost_of (m_phi jm)) 0 = Some (Some (ext_ghost OK_alg z, NoneP)) /\
            jsafeN (@OK_spec Espec) (globalenv prog) n z q jm /\
            no_locks (m_phi jm) /\
            matchfunspecs (globalenv prog) G (m_phi jm) /\
